predictor function

src/multiplier.v
@@ -1,14 +1,14 @@
 (**********************************************************************************)
 (*                                                                                *)
-(*  Standard multicycle, shift-and-add 4-bit multiplier.                          *)
+(*  multiplier.v - Shift-and-add 4-bit multiplier.                                *)
 (*                                                                                *)
 (*                   +---------------------------+                                *)
 (*                   |                           |                                *)
-(*           A -----------                 ------------- P                        *)
+(*           A -----------                 ------|------ P                        *)
 (*                   |                           |                                *)
-(*           B -----------        A*B      ------------- R                        *)
+(*           B -----------        A*B            |                                *)
 (*                   |                           |                                *)
-(*           V -----------                       |                                *)
+(*           V -----------                 ------------- R                        *)
 (*                   |                           |                                *)
 (*                   +---------------------------+                                *)
 (*                                                                                *)
@@ -22,7 +22,8 @@
 (*                                                                                *)
 (*  A specification leakage trace [t] is extracted from schedule [C] which        *)
 (*  will record the values of [A] and [valid] each cycle. On termination,         *)
-(*  the following invariant must hold [t' = f(t)].                                *)
+(*                                                                                *)
+(*                              [t' = f(t)].                                      *)
 (*                                                                                *)
 (**********************************************************************************)
 
@@ -33,8 +34,7 @@ Local Open Scope bv_scope.
 
 Ltac Zify.zify_post_hook ::= Z.div_mod_to_equations.
 
-Ltac simplify :=
-  repeat progress (intros; csimpl in *; subst).
+Ltac simplify := repeat progress (intros; csimpl in *; subst).
 
 Definition make_visible {X} (f : X) := f.
 
@@ -53,21 +53,28 @@ Infix "=?" := bv_eqb : bv_scope.
 Infix "#" := bv_zero_extend (at level 65) : bv_scope.
 Infix "||" := (bv_concat _) : bv_scope.
 
-Record Registers := mkRegisters { RA : bv 8 ; RB : bv 4 ; RCount : bv 2 ; RBusy : bv 1}.
+Notation "x ?" := (bv_odd x) : bv_scope.
+
+Record Registers :=
+  mkRegisters { r_A : bv 8 ; r_B : bv 4 ; r_cnt : bv 2 ; r_busy : bv 1}.
 
 Definition Registers0 := mkRegisters 0 0 0 0.
 
-Record In := mkIn { InA : bv 4 ; InB : bv 4 ; InValid : bv 1}.
+Record In :=
+  mkIn { in_A : bv 4 ; in_B : bv 4 ; in_valid : bv 1}.
 
 Definition In0 := mkIn 0 0 0.
 
-Record Out := mkOut { OutP : bv 8 ; OutReady : bv 1 }.
+Record Out :=
+  mkOut { out_P : bv 8 ; out_ready : bv 1 }.
 
 Definition Out0 := mkOut 0 0.
 
-Record ILeakage := mkILeak { LeakValid : bv 1 ; LeakReady : bv 1}.
+Record ILeakage :=
+  mkILeak { leak_valid : bv 1 ; leak_ready : bv 1}.
 
-Record State := mkState { R : Registers ; T : list ILeakage}.
+Record State :=
+  mkState { R : Registers ; T : list ILeakage}.
 
 Definition State0 := mkState Registers0 [].
 
@@ -75,44 +82,44 @@ Definition State0 := mkState Registers0 [].
    shift-right by one by reassembly. *)
 Definition shift_and_add (b : bv 4) (a : bv 8) : bv 8 :=
   let t0 := bv_extract 4 5 a in
-  let t1 := if bv_odd a then 5#b else 0 in
+  let t1 := if a? then 5#b else 0 in
   t0 + t1 || bv_extract 1 3 a.
 
 Definition cycle (s : State) (x : In) : State * Out :=
-  if s.(R).(RBusy) =? 0
+  if s.(R).(r_busy) =? 0
   then
-    if x.(InValid) =? 1
+    if x.(in_valid) =? 1
     then
-      let ra' := 8#x.(InA) in
-      let rb' := x.(InB) in
+      let ra' := 8#x.(in_A) in
+      let rb' := x.(in_B) in
       let rcount' := 3 in
       let rbusy' := 1 in
       let r' := mkRegisters ra' rb' rcount' rbusy' in
-      let t' := s.(T) ++ [mkILeak x.(InValid) 0 ] in
+      let t' := s.(T) ++ [mkILeak x.(in_valid) 0 ] in
       let s' := mkState r' t' in
       (s', Out0)
     else
-      let t' := s.(T) ++ [mkILeak x.(InValid) 0 ] in
+      let t' := s.(T) ++ [mkILeak x.(in_valid) 0 ] in
       let r' := s.(R) in
       let s' := mkState r' t' in
       (s', Out0)
   else
-    let ra' := shift_and_add s.(R).(RB) s.(R).(RA) in
-    let rb' := s.(R).(RB) in
-    if s.(R).(RCount) =? 0
+    let ra' := shift_and_add s.(R).(r_B) s.(R).(r_A) in
+    let rb' := s.(R).(r_B) in
+    if s.(R).(r_cnt) =? 0
     then
       let rcount' := 0 in
       let rbusy' := 0 in
       let r' := mkRegisters ra' rb' rcount' rbusy' in
-      let t' := s.(T) ++ [mkILeak x.(InValid) 1 ] in
+      let t' := s.(T) ++ [mkILeak x.(in_valid) 1 ] in
       let s' := mkState r' t' in
       let o' := mkOut ra' 1 in
       (s', o')
     else
-      let rcount' := s.(R).(RCount) - 1 in
+      let rcount' := s.(R).(r_cnt) - 1 in
       let rbusy' := 1 in
       let r' := mkRegisters ra' rb' rcount' rbusy' in
-      let t' := s.(T) ++ [mkILeak x.(InValid) 0 ] in
+      let t' := s.(T) ++ [mkILeak x.(in_valid) 0 ] in
       let s' := mkState r' t' in
       (s', Out0).
 
@@ -123,6 +130,12 @@ Fixpoint cycles (s : State) (xs : list In) : State * list Out :=
       let (s', y) := cycle s x in
       let (s'', ys) := cycles s' xs' in
       (s'', y :: ys)
+  end.
+
+Fixpoint cycles' (s : State) (xs : list In) : State :=
+  match xs with
+  | [] => s
+  | x :: xs' => cycles' (fst (cycle s x)) xs'
   end.
 
 Fixpoint repeat {A : Type} (f : A -> A) (n : nat) {struct n} : (A -> A) :=
@@ -172,7 +185,7 @@ Qed.
 
 (* Tactic for exhaustive case analysis on integers in range [0,16) *)
 (* Automatically finds variables with range hypotheses and does case analysis *)
-Ltac case_range16 :=
+Ltac by_cases16 :=
   repeat match goal with
     | [ H : (0 <= ?z < 16)%Z |- _ ] =>
         let Hz := fresh "Hcases" in
@@ -187,10 +200,7 @@ Lemma shift_and_add4'_multiplies : forall a b,
     (0 <= b < bv_modulus 4%N)%Z ->
     shift_and_add4' b a = (a * b)%Z.
 Proof.
-  intros a b Ha Hb.
-  replace (bv_modulus 4%N) with 16%Z in * by trivial.
-  rewrite Z.mul_comm.
-  case_range16.
+  intros a b Ha Hb. replace (bv_modulus 4%N) with 16%Z in * by easy. by_cases16.
 Qed.
 
 Lemma shift_and_add4_multiplies : forall (a b : bv 4),
@@ -222,51 +232,51 @@ Proof.
   apply bv_1_ind with (P := (fun b => b = 0 \/ b = 1)); intuition congruence.
 Qed.
 
-Definition busy (s : State) := s.(R).(RBusy) = 1.
-Definition finished (s : State) := s.(R).(RCount) = 0.
-Definition valid (x : In) := x.(InValid) = 1.
+Definition busy (s : State) := s.(R).(r_busy) = 1.
+Definition finished (s : State) := s.(R).(r_cnt) = 0.
+Definition valid (x : In) := x.(in_valid) = 1.
 
 Hint Extern 1 (_ = _ :> bv 1) =>
        match goal with
        | |- ?b = 0 :> bv 1 => pose proof (bv1_is_0_or_1 b); intuition
-| |- ?b = 1 :> bv 1 => pose proof (bv1_is_0_or_1 b); intuition
-end : multiplier.
+       | |- ?b = 1 :> bv 1 => pose proof (bv1_is_0_or_1 b); intuition
+       end : multiplier.
 
 Definition cycle_idle_valid s1 x s2 y : Prop :=
   ~ busy s1 -> valid x -> (s2, y) = cycle s1 x ->
-  (s2, y) = (s1 <| R := {| RA := 8#x.(InA); RB := x.(InB); RCount := 3; RBusy := 1 |} |>
-                <| T := s1.(T) ++ [{| LeakValid := 1; LeakReady := 0 |}] |>,
+  (s2, y) = (s1 <| R := {| r_A := 8#x.(in_A); r_B := x.(in_B); r_cnt := 3; r_busy := 1 |} |>
+                <| T := s1.(T) ++ [{| leak_valid := 1; leak_ready := 0 |}] |>,
              Out0).
 
 Lemma cycle_idle_valid_holds : forall s1 x s2 y, cycle_idle_valid s1 x s2 y.
 Proof.
   unfold cycle_idle_valid. simplify.
   unfold cycle in *. unfold bv_eqb in *. unfold busy in *.
-  unfold valid in *. assert (s1.(R).(RBusy) = 0) by auto with multiplier.
+  unfold valid in *. assert (s1.(R).(r_busy) = 0) by auto with multiplier.
   repeat rewrite H2 in H1. simpl in *. rewrite H0 in H1.
   simplify. inv H1. done.
 Qed.
 
 Definition cycle_idle_invalid s1 x s2 y : Prop :=
   ~ busy s1 -> ~ valid x -> (s2, y) = cycle s1 x ->
-  (s2, y) = (s1 <| T := s1.(T) ++ [{| LeakValid := 0; LeakReady := 0 |}] |>,
-                             Out0).
+  (s2, y) = (s1 <| T := s1.(T) ++ [{| leak_valid := 0; leak_ready := 0 |}] |>,
+             Out0).
 
 Lemma cycle_idle_invalid_holds : forall s1 x s2 y, cycle_idle_invalid s1 x s2 y.
 Proof.
   unfold cycle_idle_invalid. simplify.
   unfold cycle, bv_eqb, busy, valid in *.
-  assert (s1.(R).(RBusy) = 0) by auto with multiplier.
-  assert (x.(InValid) = 0) by auto with multiplier.
+  assert (s1.(R).(r_busy) = 0) by auto with multiplier.
+  assert (x.(in_valid) = 0) by auto with multiplier.
   rewrite H2, H3 in H1. simpl in *. inversion H1; clear H1.
   done.
 Qed.
 
 Definition cycle_busy_unfinished s1 x s2 y : Prop :=
   busy s1 -> ~ finished s1 -> (s2, y) = cycle s1 x ->
-  (s2, y) = (s1 <| R; RA := shift_and_add s1.(R).(RB) s1.(R).(RA) |>
-                <| R; RCount := s1.(R).(RCount) - 1 |>
-                <| T := s1.(T) ++ [{| LeakValid := x.(InValid); LeakReady := 0 |}] |>,
+  (s2, y) = (s1 <| R; r_A := shift_and_add s1.(R).(r_B) s1.(R).(r_A) |>
+                <| R; r_cnt := s1.(R).(r_cnt) - 1 |>
+                <| T := s1.(T) ++ [{| leak_valid := x.(in_valid); leak_ready := 0 |}] |>,
               Out0).
 
 Lemma cycle_busy_unfinished_holds : forall s1 x s2 y, cycle_busy_unfinished s1 x s2 y.
@@ -274,18 +284,18 @@ Proof.
   unfold cycle_busy_unfinished. simplify.
   unfold cycle, bv_eqb, busy, finished in *.
   rewrite H in H1; simpl in *.
-  destruct (bv_eq_dec 2 (RCount (R s1)) 0) as [Heq | Hneq].
+  destruct (bv_eq_dec 2 (r_cnt (R s1)) 0) as [Heq | Hneq].
   - done.
-  - inversion H1; clear H1; subst. intuition congruence.
+  - inv H1. intuition congruence.
 Qed.
 
 Definition cycle_busy_finished s1 x s2 y : Prop :=
   busy s1 -> finished s1 -> (s2, y) = cycle s1 x ->
-  (s2, y) = (s1 <| R; RA := shift_and_add s1.(R).(RB) s1.(R).(RA) |>
-                <| R; RCount := 0 |>
-                <| R; RBusy := 0 |>
-                <| T := s1.(T) ++ [{| LeakValid := x.(InValid); LeakReady := 1 |}] |>,
-                {| OutP := s2.(R).(RA); OutReady := 1 |}).
+  (s2, y) = (s1 <| R; r_A := shift_and_add s1.(R).(r_B) s1.(R).(r_A) |>
+                <| R; r_cnt := 0 |>
+                <| R; r_busy := 0 |>
+                <| T := s1.(T) ++ [{| leak_valid := x.(in_valid); leak_ready := 1 |}] |>,
+                {| out_P := s2.(R).(r_A); out_ready := 1 |}).
 
 Lemma cycle_busy_finished_holds : forall s1 x s2 y, cycle_busy_finished s1 x s2 y.
 Proof.
@@ -320,15 +330,15 @@ Ltac cycles_correct_auto :=
                         [ intuition
                         | simplify; bv_solve ]).
 
-(* Finally, with all those helper theorems out of the way, we can now prove
-     the following correctness property:
+(* Finally, with all those helper theorems out of the way, we can now prove the
+   following correctness property:
 
-     For any cycle where the circuit is idle, if a valid [a] and [b] are
-     provided, four cycles later it will produce [a *| b]. *)
+   For any cycle where the circuit is idle, if a valid [a] and [b] are provided,
+   four cycles later it will produce [a *| b]. *)
 Theorem cycles_correct : forall s s' x1 x2 x3 x4 x5 ys a b,
-    ~ busy s -> x1 = {| InA := a; InB := b; InValid := 1 |} ->
+    ~ busy s -> x1 = {| in_A := a; in_B := b; in_valid := 1 |} ->
     (s', ys) = cycles s [x1; x2; x3; x4; x5] ->
-    ys = [Out0; Out0; Out0; Out0; {| OutP := a *| b; OutReady := 1 |}].
+    ys = [Out0; Out0; Out0; Out0; {| out_P := a *| b; out_ready := 1 |}].
 Proof.
   simplify. unroll_lets.
   apply cycle_idle_valid_holds      in Hlet0; cycles_correct_auto.
@@ -339,15 +349,13 @@ Proof.
   simplify. repeat f_equal. by apply shift_and_add4_correct.
 Qed.
 
-(** NOTE knwabueze for aerbsen: I think we talked about using this definition
-      for the extraction from the list of inputs to the specification leakage.
+(* NOTE knwabueze for aerbsen: I think we talked about using this definition for
+   the extraction from the list of inputs to the specification leakage.
 
-    {[
-        Definition SLeakage := bv 4.
+   {[ Definition SLeakage := bv 4.
 
-        Definition extract : list In -> list SLeakage :=
-          flat_map (fun i => if i.(InValid) =? 1 then [i.(InA)] else []).
-    ]}
+      Definition extract : list In -> list SLeakage := flat_map (fun i => if
+        i.(in_valid) =? 1 then [i.(in_A)] else []). ]}
 
     However, I think this original definition is problematic. The predictor
     function would need to know whether or not a value for [A] was provided on
@@ -356,9 +364,61 @@ Qed.
 Definition SLeakage := option (bv 4).
 
 Definition extract : list In -> list SLeakage :=
-  map (fun x => if x.(InValid) =? 1 then Some x.(InA) else None).
+  map (fun x => if x.(in_valid) =? 1 then Some x.(in_A) else None).
 
-Theorem cycles_ct : exists (predictor : list SLeakage -> list ILeakage),
-  forall (xs : list In) (ys : list Out) (s : State),
-    (s, ys) = cycles State0 xs -> s.(T) = (predictor ∘ extract) xs.
+(* Predictor function which uses the prefix of the specification leakage trace
+   to predict the next item in the implementation leakage trace. *)
+Definition update_st (st : option nat * bool) (s : SLeakage) :=
+  match st with
+  | (Some (S n), _) =>
+      match s with
+      | Some _ => (Some n, true)
+      | None => (Some n, false)
+      end
+  | (Some O, _) =>
+      match s with
+      | Some _ => (None, true)
+      | None => (None, false)
+      end
+  | (None, _) =>
+      match s with
+      | Some _ => (Some 4%nat, true)
+      | None => (None, false)
+      end
+  end.
+
+Fixpoint predict_next' (prefix : list SLeakage) (st : option nat * bool) : ILeakage :=
+  match prefix with
+  | [] =>
+      match st with
+      | (None  , v) => {| leak_valid := bool_to_bv 1 v; leak_ready := 0 |}
+      | (Some O, v) => {| leak_valid := bool_to_bv 1 v; leak_ready := 1 |}
+      | (Some _, v) => {| leak_valid := bool_to_bv 1 v; leak_ready := 0 |}
+      end
+  | p :: ps => predict_next' ps (update_st st p)
+  end.
+
+Definition predict_next prefix := predict_next' prefix (None, false).
+
+Fixpoint predict' prefix xs :=
+  match xs with
+  | [] => []
+  | x :: xs' => predict_next (prefix ++ [x]) :: predict' (prefix ++ [x]) xs'
+  end.
+
+Definition predict xs := predict' [] xs.
+
+(* First, we need a helper lemma that talks about one cycle's behavior on a the
+   implementation leakage trace. This follows by doing cases analysis on the
+   four fundamental outcomes that may happen on a cycle:
+
+   1. The circuit is idle and recieves an invalid input.
+   2. The circuit is idle and recieves a valid input.
+   3. The circuit is busy, but r_cnt > 0.
+   4. The circuit is busy, but r_cnt = 0. *)
+
+Theorem cycles_ct : exists f, forall xs ys s,
+    ys = extract xs ->
+    s = cycles' State0 xs ->
+    s.(T) = f ys.
 Admitted.
